might need lemmas: https://rise4fun.com/Dafny/tutorial/Lemmas

dp/lis.dfy
@@ -4,16 +4,63 @@ reads a
     forall i, j :: 0 <= i < j < a.Length ==> a[i] < a[j]
 }
 
+predicate increasing(a: array<int>) 
+reads a
+{
+    forall i, j :: 0 <= i < j < a.Length ==> a[i] <= a[j]
+}
+
 predicate subsetOf(x: array<int>, y: array<int>)
 reads x, y
 {
     multiset(y[..]) * multiset(x[..]) == multiset(x[..])
 }
 
-method computeLIS(a: array<int>) returns (lis: array<int>) 
-ensures lis.Length <= a.Length
-ensures strictlyIncreasing(lis)
-ensures subsetOf(lis, a)
+method computeLIS(a: array<int>) returns (lisN: int) 
+requires a.Length > 0
+ensures 0 <= lisN <= a.Length
 {
-    return lis;
+    var n := a.Length;
+    if n < 3 { return 1; }
+    if n == 0 { return 0; }
+
+    var lis := new int[n];
+    var i, j := 1, 1;
+
+    while i < n 
+    invariant 0 < j <= i <= n
+    decreases n - i 
+    {
+        lis[i] := 1;
+
+        while j < i - 1 
+        invariant 0 < j <= i
+        decreases i - j - 1 
+        {
+            if a[j] < a[i] && lis[i] < lis[j] {
+                lis[i] := 1 + lis[j];
+            }
+            j := j + 1;
+        }
+        i := i + 1;
+    }
+
+    var max := 1;
+    var k := 2;
+
+    while k < n
+    invariant 0 < max <= k <= n
+    decreases n - k 
+    {
+        if lis[k] > lis[max] {
+            max := k;
+        }
+        k := k + 1;
+    }
+
+    assert max > 0;
+    assert max <= lis.Length;
+   //assert increasing(lis);
+
+    return lis[max];
 }
